Add basic semantics

S5/language.lean
@@ -1,14 +1,16 @@
 inductive form where 
-  | atom : form 
-  | neg : form → form 
+  | atom : Nat → form 
+  | bot : form
   | impl : form → form → form 
   | box : form → form 
 
 set_option quotPrecheck false
 
-notation:40 "¬"p => form.neg p 
+notation:40 "¬"p => form.impl p (form.bot)
 infix:50 "→" => form.impl 
 notation p "∧" q => ¬(p → (form.neg q))
 notation p "∨" q => ((form.neg p) ∧ (form.neg q))
 prefix:80 "□" => form.box 
 notation "⋄"p => ¬(□(¬p))
+notation "⊤" => ¬ form.bot 
+notation "⊥" => form.bot
