S5/sematics/basic.lean
@@ -1,0 +1,26 @@
+import S5.context 
+
+open Classical 
+
+def world := ctx 
+
+-- Kripke models
+structure model where
+  worlds : List world
+  access : world → world → Bool
+  val : Nat → world → Bool
+  refl : (∀ w, w ∈ worlds) → access w w = True
+  symm : (∀ w, w ∈ worlds) → (∀ v, v ∈ worlds) → access w v = True → access v w = True
+  trans : (∀ w, w ∈ worlds) → (∀ v, v ∈ worlds) → (∀ u, u ∈ worlds) → access w v = True → access v u = True → access w u = True
+
+
+noncomputable def forces_form (M : model) : form → world → Bool
+| (form.atom p) => fun w => M.val p w 
+| (form.bot) => fun w => False 
+| (form.impl p q) => fun w => (!(forces_form M p w) || (forces_form M q w)) 
+| (form.box p) => fun w => 
+    if (∀ v , (v ∈ M.worlds) → (w ∈ M.worlds) → (M.access w v = True) → (forces_form M p v = True))
+      then True 
+    else False
+
+notation M "," w "⊩" p => forces_form M p w
